Define loops like Hurd and prove some of their properties (#95)
This is a step towards a proper definition of while loops.
Previously, we used a recursive definition, which needed an `assume
false` for termination.
This PR changes it to (almost) Hurd's definition, but with a small
modification because Dafny does not have an `arb` value like HOL.

<small>By submitting this pull request, I confirm that my contribution
is made under the terms of the [MIT
license](https://github.com/dafny-lang/dafny/blob/master/LICENSE.txt).</small>

src/ProbabilisticProgramming/Loops.dfy
@@ -14,73 +14,72 @@ module Loops {
   ************/
 
   // Definition 37
-  function WhileCut<A>(condition: A -> bool, body: A -> Monad.Hurd<A>, n: nat, init: A): Monad.Hurd<A> {
-    if n == 0 then
+  function WhileCut<A>(condition: A -> bool, body: A -> Monad.Hurd<A>, init: A, fuel: nat): Monad.Hurd<A> {
+    if fuel == 0 || !condition(init) then
       Monad.Return(init)
-    else (
-           if condition(init) then
-             Monad.Bind(body(init), (a: A) => WhileCut(condition, body, n-1, a))
-           else
-             Monad.Return(init)
-         )
+    else
+      Monad.Bind(body(init), (init': A) => WhileCut(condition, body, init', fuel - 1))
+  }
+
+  ghost predicate WhileCutTerminates<A>(condition: A -> bool, body: A -> Monad.Hurd<A>, init: A, s: Rand.Bitstream) {
+    exists fuel: nat :: WhileCutTerminatesWithFuel(condition, body, init, s)(fuel)
+  }
+
+  ghost function WhileCutTerminatesWithFuel<A>(condition: A -> bool, body: A -> Monad.Hurd<A>, init: A, s: Rand.Bitstream): nat -> bool {
+    (fuel: nat) => !condition(WhileCut(condition, body, init, fuel)(s).0)
   }
 
   // Definition 39 / True iff Prob(iset s | While(condition, body, a)(s) terminates) == 1
-  ghost predicate WhileTerminates<A(!new)>(condition: A -> bool, body: A -> Monad.Hurd<A>) {
-    var p := (a: A) =>
-               (s: Rand.Bitstream) => exists n :: !condition(WhileCut(condition, body, n, a)(s).0);
-    forall a :: Quantifier.AlmostSurely(p(a))
+  ghost predicate WhileTerminatesAlmostSurely<A(!new)>(condition: A -> bool, body: A -> Monad.Hurd<A>) {
+    var p := (init: A) =>
+               (s: Rand.Bitstream) => WhileCutTerminates(condition, body, init, s);
+    forall init :: Quantifier.AlmostSurely(p(init))
   }
 
-  // Theorem 38
-  function While<A>(condition: A -> bool, body: A -> Monad.Hurd<A>, init: A): (f: Monad.Hurd<A>)
-    requires WhileTerminates(condition, body)
+  // Equation (3.25)
+  ghost function While<A>(condition: A -> bool, body: A -> Monad.Hurd<A>, init: A): (f: Monad.Hurd<A>)
   {
-    assume {:axiom} false; // assume termination
-    if condition(init) then
-      Monad.Bind(body(init), (a': A) => While(condition, body, a'))
-    else
-      Monad.Return(init)
+    (s: Rand.Bitstream) =>
+      if WhileCutTerminates(condition, body, init, s)
+      then
+        var fuel := LeastFuel(condition, body, init, s);
+        WhileCut(condition, body, init, fuel)(s)
+      else
+        // In HOL, Hurd returns `arb` here, which is not possible in Dafny.
+        (init, s)
   }
 
-  method WhileImperative<A>(condition: A -> bool, body: A -> Monad.Hurd<A>, init: A, s: Rand.Bitstream) returns (t: (A, Rand.Bitstream))
-    requires WhileTerminates(condition, body)
-    ensures While(condition, body, init)(s) == t
-    decreases *
+  ghost function LeastFuel<A>(condition: A -> bool, body: A -> Monad.Hurd<A>, init: A, s: Rand.Bitstream): (fuel: nat)
+    requires WhileCutTerminates(condition, body, init, s)
+    ensures WhileCutTerminatesWithFuel(condition, body, init, s)(fuel)
+    ensures forall fuel': nat :: WhileCutTerminatesWithFuel(condition, body, init, s)(fuel') ==> fuel <= fuel'
   {
-    while condition(init)
-      decreases *
-    {
-      var (a, s) := body(init)(s);
-    }
-    return (init, s);
+    var fuelBound :| WhileCutTerminatesWithFuel(condition, body, init, s)(fuelBound);
+    Least(WhileCutTerminatesWithFuel(condition, body, init, s), fuelBound)
   }
 
-  method WhileImperativeAlternative<A>(condition: A -> bool, body: A -> Monad.Hurd<A>, init: A, s: Rand.Bitstream) returns (t: (A, Rand.Bitstream))
-    requires WhileTerminates(condition, body)
-    ensures While(condition, body, init)(s) == t
-    decreases *
+  ghost function Least(property: nat -> bool, bound: nat, start: nat := 0): (l: nat)
+    decreases bound - start
+    requires start <= bound
+    requires property(bound)
+    ensures property(l)
+    ensures start <= l <= bound
+    ensures forall n: nat | start <= n :: property(n) ==> l <= n
   {
-    while true
-      decreases *
-    {
-      if !condition(init) {
-        return (init, s);
-      } else {
-        var (a, s) := body(init)(s);
-      }
-    }
+    if start == bound || property(start)
+    then start
+    else Least(property, bound, start + 1)
   }
 
-  ghost predicate UntilTerminates<A(!new)>(proposal: Monad.Hurd<A>, accept: A -> bool) {
+  ghost predicate UntilTerminatesAlmostSurely<A(!new)>(proposal: Monad.Hurd<A>, accept: A -> bool) {
     var reject := (a: A) => !accept(a);
     var body := (a: A) => proposal;
-    WhileTerminates(reject, body)
+    WhileTerminatesAlmostSurely(reject, body)
   }
 
   // Definition 44
-  function Until<A>(proposal: Monad.Hurd<A>, accept: A -> bool): (f: Monad.Hurd<A>)
-    requires UntilTerminates(proposal, accept)
+  ghost function Until<A>(proposal: Monad.Hurd<A>, accept: A -> bool): (f: Monad.Hurd<A>)
+    requires UntilTerminatesAlmostSurely(proposal, accept)
     ensures
       var reject := (a: A) => !accept(a);
       var body := (a: A) => proposal;
@@ -89,16 +88,6 @@ module Loops {
     var reject := (a: A) => !accept(a);
     var body := (a: A) => proposal;
     Monad.Bind(proposal, (a: A) => While(reject, body, a))
-  }
-
-  method UntilImperative<A>(proposal: Monad.Hurd<A>, accept: A -> bool, s: Rand.Bitstream) returns (t: (A, Rand.Bitstream))
-    requires UntilTerminates(proposal, accept)
-    ensures t == Until(proposal, accept)(s)
-    decreases *
-  {
-    var reject := (a: A) => !accept(a);
-    var body := (a: A) => proposal;
-    t := WhileImperative(reject, body, proposal(s).0, proposal(s).1);
   }
 
   function WhileLoopExitsAfterOneIteration<A(!new)>(body: A -> Monad.Hurd<A>, condition: A -> bool, init: A): (Rand.Bitstream -> bool) {
@@ -111,15 +100,15 @@ module Loops {
       accept(proposal(s).0)
   }
 
-  function UntilLoopResultIsAccepted<A>(proposal: Monad.Hurd<A>, accept: A -> bool): (Rand.Bitstream -> bool)
-    requires UntilTerminates(proposal, accept)
+  ghost function UntilLoopResultIsAccepted<A>(proposal: Monad.Hurd<A>, accept: A -> bool): (Rand.Bitstream -> bool)
+    requires UntilTerminatesAlmostSurely(proposal, accept)
   {
     (s: Rand.Bitstream) =>
       accept(Until(proposal, accept)(s).0)
   }
 
   ghost function UntilLoopResultHasProperty<A>(proposal: Monad.Hurd<A>, accept: A -> bool, property: A -> bool): iset<Rand.Bitstream>
-    requires UntilTerminates(proposal, accept)
+    requires UntilTerminatesAlmostSurely(proposal, accept)
   {
     iset s | property(Until(proposal, accept)(s).0)
   }
@@ -139,15 +128,118 @@ module Loops {
    Lemmas
   *******/
 
+  lemma LeastFuelUnroll<A>(condition: A -> bool, body: A -> Monad.Hurd<A>, init: A, s: Rand.Bitstream, init': A, s': Rand.Bitstream, fuel': nat)
+    requires WhileCutTerminates(condition, body, init', s')
+    requires LeastFuel(condition, body, init', s') == fuel'
+    requires condition(init)
+    requires body(init)(s) == (init', s')
+    ensures WhileCutTerminates(condition, body, init, s)
+    ensures LeastFuel(condition, body, init, s) == fuel' + 1
+  {
+    assert WhileCutTerminates(condition, body, init, s) by {
+      WhileCutTerminatesWithFuelUnroll(condition, body, init, s, init', s', fuel');
+    }
+    var fuel := LeastFuel(condition, body, init, s);
+    assert fuel == fuel' + 1 by {
+      WhileCutTerminatesWithFuelUnroll(condition, body, init, s, init', s', fuel');
+      WhileCutTerminatesWithFuelUnroll(condition, body, init, s, init', s', fuel - 1);
+    }
+  }
+
+  lemma WhileCutUnroll<A>(condition: A -> bool, body: A -> Monad.Hurd<A>, init: A, s: Rand.Bitstream, init': A, s': Rand.Bitstream, fuel: nat)
+    requires condition(init)
+    requires body(init)(s) == (init', s')
+    ensures WhileCut(condition, body, init, fuel + 1)(s) == WhileCut(condition, body, init', fuel)(s')
+  {}
+
+
+  lemma WhileCutTerminatesWithFuelUnroll<A>(condition: A -> bool, body: A -> Monad.Hurd<A>, init: A, s: Rand.Bitstream, init': A, s': Rand.Bitstream, fuel: nat)
+    requires condition(init)
+    requires body(init)(s) == (init', s')
+    ensures WhileCutTerminatesWithFuel(condition, body, init, s)(fuel + 1) == WhileCutTerminatesWithFuel(condition, body, init', s')(fuel)
+  {}
+
+  lemma WhileUnrollIfConditionSatisfied<A>(condition: A -> bool, body: A -> Monad.Hurd<A>, init: A, s: Rand.Bitstream, init': A, s': Rand.Bitstream, loop: (A, Rand.Bitstream), unrolled: (A, Rand.Bitstream))
+    requires WhileCutTerminates(condition, body, init, s)
+    requires condition(init)
+    requires body(init)(s) == (init', s')
+    requires loop == While(condition, body, init)(s)
+    requires unrolled == While(condition, body, init')(s')
+    ensures loop == unrolled
+  {
+    var fuel: nat := LeastFuel(condition, body, init, s);
+    assert fuel >= 1;
+    var fuel': nat := fuel - 1;
+    assert WhileCutTerminatesWithFuel(condition, body, init', s')(fuel');
+    assert WhileCutTerminates(condition, body, init', s');
+    var minFuel: nat := LeastFuel(condition, body, init', s');
+    assert minFuel == fuel' by {
+      LeastFuelUnroll(condition, body, init, s, init', s', minFuel);
+    }
+    assert loop == unrolled by {
+      calc {
+        loop;
+        WhileCut(condition, body, init, fuel)(s);
+        { WhileCutUnroll(condition, body, init, s, init', s', fuel'); }
+        WhileCut(condition, body, init', fuel')(s');
+        unrolled;
+      }
+    }
+  }
+
+  lemma WhileUnrollIfTerminates<A>(condition: A -> bool, body: A -> Monad.Hurd<A>, init: A, s: Rand.Bitstream, fuel: nat, loop: (A, Rand.Bitstream), unrolled: (A, Rand.Bitstream))
+    requires WhileCutTerminates(condition, body, init, s)
+    requires fuel == LeastFuel(condition, body, init, s)
+    requires loop == While(condition, body, init)(s)
+    requires unrolled == (if condition(init) then Monad.Bind(body(init), (init': A) => While(condition, body, init')) else Monad.Return(init))(s)
+    ensures loop == unrolled
+  {
+    if condition(init) {
+      var (init', s') := body(init)(s);
+      calc {
+        loop;
+        { WhileUnrollIfConditionSatisfied(condition, body, init, s, init', s', loop, unrolled); }
+        While(condition, body, init')(s');
+        unrolled;
+      }
+    } else {
+      calc {
+        loop;
+        (init, s);
+        unrolled;
+      }
+    }
+  }
+
+  // Theorem 38
+  lemma WhileUnroll<A>(condition: A -> bool, body: A -> Monad.Hurd<A>, init: A, s: Rand.Bitstream)
+    requires WhileTerminatesAlmostSurely(condition, body)
+    ensures While(condition, body, init)(s) == (if condition(init) then Monad.Bind(body(init), (init': A) => While(condition, body, init')) else Monad.Return(init))(s)
+  {
+    var loop := While(condition, body, init)(s);
+    var unrolled := (if condition(init) then Monad.Bind(body(init), (init': A) => While(condition, body, init')) else Monad.Return(init))(s);
+    assert loop == unrolled by {
+      if WhileCutTerminates(condition, body, init, s) {
+        var fuel: nat := LeastFuel(condition, body, init, s);
+        WhileUnrollIfTerminates(condition, body, init, s, fuel, loop, unrolled);
+      } else {
+        // In this case, equality does not hold in Dafny.
+        // Hurd avoids this problem in HOL by having `While` return `arb` (an arbitrary value) in this case.
+        // That's not possible in Dafny, so we must resort to `assume false`.
+        assume {:axiom} false;
+      }
+    }
+  }
+
   lemma EnsureUntilTerminates<A(!new)>(proposal: Monad.Hurd<A>, accept: A -> bool)
     requires Independence.IsIndep(proposal)
     requires Quantifier.WithPosProb((s: Rand.Bitstream) => accept(proposal(s).0))
-    ensures UntilTerminates(proposal, accept)
+    ensures UntilTerminatesAlmostSurely(proposal, accept)
   {
     var reject := (a: A) => !accept(a);
     var body := (a: A) => proposal;
     var proposalIsAccepted := (s: Rand.Bitstream) => accept(proposal(s).0);
-    assert UntilTerminates(proposal, accept) by {
+    assert UntilTerminatesAlmostSurely(proposal, accept) by {
       forall a: A ensures Independence.IsIndep(body(a)) {
         assert body(a) == proposal;
       }
@@ -155,7 +247,7 @@ module Loops {
         assert Quantifier.WithPosProb(proposalIsAccepted);
         assert (iset s | proposalIsAccepted(s)) == (iset s | WhileLoopExitsAfterOneIteration(body, reject, a)(s));
       }
-      assert WhileTerminates(reject, body) by {
+      assert WhileTerminatesAlmostSurely(reject, body) by {
         EnsureWhileTerminates(reject, body);
       }
     }
@@ -165,13 +257,13 @@ module Loops {
   lemma {:axiom} EnsureWhileTerminates<A(!new)>(condition: A -> bool, body: A -> Monad.Hurd<A>)
     requires forall a :: Independence.IsIndep(body(a))
     requires forall a :: Quantifier.WithPosProb(WhileLoopExitsAfterOneIteration(body, condition, a))
-    ensures WhileTerminates(condition, body)
+    ensures WhileTerminatesAlmostSurely(condition, body)
 
   // Theorem 45 (wrong!) / PROB_BERN_UNTIL (correct!)
   lemma {:axiom} UntilProbabilityFraction<A>(proposal: Monad.Hurd<A>, accept: A -> bool, d: A -> bool)
     requires Independence.IsIndep(proposal)
     requires Quantifier.WithPosProb(ProposalIsAccepted(proposal, accept))
-    ensures UntilTerminates(proposal, accept)
+    ensures UntilTerminatesAlmostSurely(proposal, accept)
     ensures
       && UntilLoopResultHasProperty(proposal, accept, d) in Rand.eventSpace
       && ProposalIsAcceptedAndHasProperty(proposal, accept, d) in Rand.eventSpace
@@ -180,42 +272,54 @@ module Loops {
       && Rand.prob(UntilLoopResultHasProperty(proposal, accept, d)) == Rand.prob(ProposalIsAcceptedAndHasProperty(proposal, accept, d)) / Rand.prob(ProposalAcceptedEvent(proposal, accept))
 
   // Equation (3.39)
-  lemma {:axiom} UntilAsBind<A(!new)>(proposal: Monad.Hurd<A>, accept: A -> bool, s: Rand.Bitstream)
+  lemma UntilUnroll<A(!new)>(proposal: Monad.Hurd<A>, accept: A -> bool, s: Rand.Bitstream)
     requires Independence.IsIndep(proposal)
-    requires Quantifier.WithPosProb(ProposalIsAccepted(proposal, accept))
-    ensures UntilTerminates(proposal, accept)
-    ensures Until(proposal, accept) == Monad.Bind(proposal, (x: A) => if accept(x) then Monad.Return(x) else Until(proposal, accept))
+    requires UntilTerminatesAlmostSurely(proposal, accept)
+    ensures Until(proposal, accept)(s) == Monad.Bind(proposal, (x: A) => if accept(x) then Monad.Return(x) else Until(proposal, accept))(s)
+  {
+    var reject := (a: A) => !accept(a);
+    var body := (a: A) => proposal;
+    var (init, s') := proposal(s);
+    WhileUnroll(reject, body, init, s');
+  }
 
   // Equation (3.40)
   lemma EnsureUntilTerminatesAndForAll<A(!new)>(proposal: Monad.Hurd<A>, accept: A -> bool)
     requires Independence.IsIndep(proposal)
     requires Quantifier.WithPosProb(ProposalIsAccepted(proposal, accept))
-    ensures UntilTerminates(proposal, accept)
+    ensures UntilTerminatesAlmostSurely(proposal, accept)
     ensures Quantifier.AlmostSurely(UntilLoopResultIsAccepted(proposal, accept))
   {
     EnsureUntilTerminates(proposal, accept);
     assume {:axiom} Quantifier.AlmostSurely(UntilLoopResultIsAccepted(proposal, accept)); // add later
   }
 
+  lemma WhileCutIsIndep<A(!new)>(condition: A -> bool, body: A -> Monad.Hurd<A>, init: A, fuel: nat)
+    requires forall a: A :: Independence.IsIndep(body(a))
+    ensures Independence.IsIndep(WhileCut(condition, body, init, fuel))
+  {
+    if fuel == 0 || !condition(init) {
+      Independence.ReturnIsIndep(init);
+    } else {
+      forall init': A ensures Independence.IsIndep(WhileCut(condition, body, init', fuel - 1)) {
+        WhileCutIsIndep(condition, body, init', fuel - 1);
+      }
+      Independence.BindIsIndep(body(init), init' => WhileCut(condition, body, init', fuel - 1));
+    }
+  }
+
   lemma WhileIsIndep<A(!new)>(condition: A -> bool, body: A -> Monad.Hurd<A>, init: A)
     requires forall a: A :: Independence.IsIndep(body(a))
-    requires WhileTerminates(condition, body)
+    requires WhileTerminatesAlmostSurely(condition, body)
     ensures Independence.IsIndep(While(condition, body, init))
   {
-    if condition(init) {
-      forall a ensures Independence.IsIndep(While(condition, body, a)) {
-        assume {:axiom} false; // circular reasoning, rewrite this proof
-        WhileIsIndep(condition, body, a);
-      }
-      Independence.IndepFnIsCompositional(body(init), a => While(condition, body, a));
-    } else {
-      Independence.ReturnIsIndep(init);
-    }
+    // To prove this, we need a definition of Independence.IsIndep
+    assume {:axiom} false;
   }
 
   lemma UntilIsIndep<A(!new)>(proposal: Monad.Hurd<A>, accept: A -> bool)
     requires Independence.IsIndep(proposal)
-    requires UntilTerminates(proposal, accept)
+    requires UntilTerminatesAlmostSurely(proposal, accept)
     ensures Independence.IsIndep(Until(proposal, accept))
   {
     var reject := (a: A) => !accept(a);
@@ -223,6 +327,6 @@ module Loops {
     forall init: A {
       WhileIsIndep(reject, body, init);
     }
-    Independence.IndepFnIsCompositional(proposal, (init: A) => While(reject, body, init));
+    Independence.BindIsIndep(proposal, (init: A) => While(reject, body, init));
   }
 }
